wip

x86/Asmrel.v
@@ -4,17 +4,50 @@ Require Import Locations Stacklayout Conventions.
 Require Import Mach LanguageInterface CKLR.
 Require Import Asm.
 
-Definition genv_match p R w: relation genv :=
-  (match_stbls R w) !! (fun se => Genv.globalenv se p).
+Section PROG.
+  Context (p: program).
+  Definition genv_match R w: relation genv :=
+    (match_stbls R w) !! (fun se => Genv.globalenv se p).
 
-Inductive state_match R w: rel (block * Asm.state) (block * Asm.state) :=
-| state_rel: forall (rs1 rs2: regset) m1 m2 b1 b2 nb1 nb2,
-    (forall r: preg, Val.inject (mi R w) (rs1 r) (rs2 r)) ->
-    match_mem R w m1 m2 ->
-    b1 = b2 ->
-    nb1 = Mem.nextblock m1 ->
-    nb2 = Mem.nextblock m2 ->
-    state_match R w (nb1, Asm.State rs1 m1 b1) (nb2, Asm.State rs2 m2 b2).
+  Lemma match_prog {C} `{!Linking.Linker C} (c: C):
+    Linking.match_program_gen (fun _ => eq) eq c p p.
+  Proof.
+    repeat apply conj; auto.
+    induction (AST.prog_defs p) as [ | [id [f|v]] defs IHdefs];
+      repeat (econstructor; eauto).
+    - apply Linking.linkorder_refl.
+    - destruct v; constructor; auto.
+  Qed.
+  
+  Global Instance find_funct_inject R w ge1 v1 ge2 v2 f:
+    Transport (genv_match R w * Val.inject (mi R w)) (ge1, v1) (ge2, v2)
+              (Genv.find_funct ge1 v1 = Some f)
+              (Genv.find_funct ge2 v2 = Some f).
+  Proof.
+    intros [Hge Hv] Hf. cbn in *.
+    destruct Hge. apply match_stbls_proj in H. cbn in Hf.
+    edestruct @Genv.find_funct_match as (?&?&?&?&?); eauto using (match_prog tt).
+    cbn in *. subst. auto.
+  Qed.
+
+  Global Instance genv_match_acc R:
+    Monotonic (genv_match R) (wacc R ++> subrel).
+  Proof.
+    intros w w' Hw' _ _ [se1 se2 Hge].
+    eapply (match_stbls_acc R w w') in Hge; eauto.
+    eapply (rel_push_rintro (fun se => Genv.globalenv se p) (fun se => Genv.globalenv se p));
+      eauto.
+  Qed.
+
+  Inductive state_match R w: rel (block * Asm.state) (block * Asm.state) :=
+  | state_rel: forall (rs1 rs2: regset) m1 m2 b1 b2 nb1 nb2,
+      (forall r: preg, Val.inject (mi R w) (rs1 r) (rs2 r)) ->
+      match_mem R w m1 m2 ->
+      b1 = b2 ->
+      nb1 = Mem.nextblock m1 ->
+      nb2 = Mem.nextblock m2 ->
+      state_match R w (nb1, Asm.State rs1 m1 b1) (nb2, Asm.State rs2 m2 b2).
+End PROG.
 
 Lemma semantics_asm_rel p R:
   forward_simulation (cc_asm R) (cc_asm R) (Asm.semantics p) (Asm.semantics p).
@@ -31,25 +64,58 @@ Proof.
     cbn. eapply Genv.is_internal_match; eauto.
     + repeat apply conj; auto.
       induction (prog_defs p) as [ | [id [f|v]] defs IHdefs]; repeat (econstructor; eauto).
-      * admit.                  (* match_fundef *)
-      * admit.                  (* match_varinfo *)
+      * instantiate (2 := fun _ => eq). reflexivity.
+      * instantiate (1 := eq). destruct v. constructor. auto.
     + eapply match_stbls_proj; auto.
-    + admit.                    (* match_fundef *)
+    + intros. rewrite H. auto.
     + admit.                    (* PC <> Vundef *)
-  - intros [rs1 m1] [rs2 m2] [nb1 s1] Hs [Hq Hnb].
+  - intros [rs1 m1] [rs2 m2] [nb1 s1] Hs [Hq Hnb]. inv Hs. inv Hq.
     assert (Hge: genv_match p R w (Genv.globalenv se1 p) (Genv.globalenv se2 p)).
     {
       cut (match_stbls R w (Genv.globalenv se1 p) (Genv.globalenv se2 p)); eauto.
       eapply (rel_push_rintro (fun se => Genv.globalenv se p) (fun se => Genv.globalenv se p)).
     }
-    destruct s1.
-    exists (Mem.nextblock m2, State rs2 m2 b).
+    assert (Hs': Genv.find_funct (Genv.globalenv se2 p) (rs2 PC) = Some (Internal f)).
+    {
+      specialize (H PC).
+      transport_hyps. assumption.
+    }
+    assert (Hrsp: rs2 RSP <> Vundef).
+    {
+      specialize (H RSP).
+      destruct H; congruence.
+    }
+    assert (Hra: rs2 RA <> Vundef).
+    {
+      specialize (H RA).
+      destruct H; congruence.
+    }
+    exists (Mem.nextblock m2, State rs2 m2 true).
     repeat apply conj; auto.
-    + admit.                    (* initial state *)
-    + admit.                    (* match *)
-  - intros [nb1 s1] [nb2 s2] [rs1 m1] Hm H.
-    admit.                      (* final state *)
-  - admit.                      (* external call *)
+    + econstructor. eassumption. assumption. assumption.
+    + cbn. esplit. split. rauto.
+      split. cbn. auto. cbn. constructor. apply H. apply H0. auto. auto. auto.
+  - intros [nb1 s1] [nb2 s2] [rs1 m1] (w' & Hw' & Hge & Hs) H. cbn in *.
+    inv H. inv Hs.
+    eexists. split. econstructor.
+    exists w'. split. apply Hw'. constructor. assumption. assumption.
+  - intros [nb1 s1] [nb2 s2] qx1 (w' & Hw' & Hge & Hs) H. cbn in *.
+    inv H. inv Hs.
+    assert (Hff: Genv.find_funct (Genv.globalenv se2 p) (rs2 PC) = Some (External (EF_external id sg))).
+    {
+      specialize (H6 PC).
+      transport_hyps. auto.
+    }
+    eexists w', _. repeat apply conj.
+    econstructor. apply Hff. constructor. auto. auto. rauto.
+    intros [rrs1 rm1] [rrs2 rm2] [rb1 rs1] (w'' & Hw'' & Hr) [Hae ?].
+    inv Hae.
+    eexists. repeat apply conj. instantiate (1 := (_, _)). cbn.
+    split. econstructor. admit.
+    reflexivity. exists w''. assert (Hw: w ~> w'). rauto.
+    split. rauto.
+    split; cbn.
+    admit.                      (* external call *)
   - admit.                      (* step *)
   - apply well_founded_ltof.
     
